Working on elim_let theorem
Have related theorem stated
Have proof structure outline
Worked on generic lemma but prob dont do
Need to prove syntax, alpha, and trans relation

src/proofs/ElimLet.v
@@ -82,35 +82,236 @@ Definition lift_trans (f: task_hd -> errState (CoqBigInt.t * hashcons_full) task
 Definition elim_let : trans_errst task := lift_trans elim_let_aux.
 Set Bullet Behavior "Strict Subproofs".
 (*Soundness*)
-Require Import Relations ErrStateHoare StateInvar Soundness.
+Require Import Task Relations ErrStateHoare StateInvar Soundness.
 Require Import eliminate_let.
 Check trans_errst.
 
+(*TODO: move*)
+(*We can remove a pure proposition from a precondition of errst_spec*)
+Definition errst_spec_pure_pre {St A: Type} (P1: St -> Prop) (P2: Prop) (s: errState St A) Q:
+  (P2 -> errst_spec P1 s Q) ->
+  errst_spec (fun x => P1 x /\ P2) s Q.
+Proof.
+  unfold errst_spec.
+  intros Hspec i b [Hp1 Hp2']. auto.
+Qed.
+
+(*[eval_task_goal] is annoying. This lets us rewrite it in terms of [find_goal] and relate the formulas*)
+Lemma eval_task_find_goal (tsk: task_hd) (f: formula):
+  eval_task_goal tsk = Some f <->
+  exists f1 pr, find_goal (Some tsk) = Some (pr, f1) /\ eval_fmla f1 = Some f.
+Proof.
+  unfold eval_task_goal, eval_tdecl_goal, eval_tdecl_node_aux, eval_decl_goal.
+  unfold find_goal. simpl.
+  destruct (td_node_of (task_decl tsk)) as [d | | |] eqn : Htd; try solve[split; intros; destruct_all; discriminate].
+  unfold get_goal.
+  destruct (d_node d) as [| | | | | [[k pr] f1]] eqn : Hd; try solve[split; intros; destruct_all; discriminate].
+  simpl in *. destruct k; try solve[split; intros; destruct_all; discriminate].
+  split.
+  - intros Heval. exists f1. exists pr. auto.
+  - intros [f2 [pr1 [Hsome Heval]]]. inversion Hsome; subst; auto.
+Qed.
+
+Require Import Alpha.
+
+(*Another attempt*)
+
+(*Lemma errst_spec_goal {St: Type} (tr: errState St TaskDefs.task) (fr: term_c -> errState St term_c) 
+  (f: formula -> formula)
+  (gamma gamma1: context)
+  (delta delta1: list (string * formula))
+  (goal goal1: formula)
+  (tsk1' : task_hd)
+  (*(gamma, delta, goal) is eval of tsk1*)
+  (Hgamma : eval_task_ctx tsk1' = Some gamma)
+  (Hdelta : eval_task_hyps tsk1' = Some delta)
+  (Hgoal : eval_task_goal tsk1' = Some goal)
+  (*Two tasks are alpha equivalent*)
+  (Halpha: a_equiv_task (gamma, delta, goal) (gamma1, delta1, goal1))
+  
+  errst_spec P1 (tr
+  
+
+
+
+gamma1 : context
+delta1 : list (string * formula)
+goal1 : formula
+gamma : context
+tsk1' : task_hd
+Hgamma : eval_task_ctx tsk1' = Some gamma
+delta : list (string * formula)
+Hdelta : eval_task_hyps tsk1' = Some delta
+goal : formula
+d : decl
+Htd : td_node_of (task_decl tsk1') = Decl d
+pr : prsymbol
+f1 : term_c
+Hd : d_node d = Dprop (Pgoal, pr, f1)
+Hgoal : eval_fmla f1 = Some goal
+Halphag : a_equiv_ctx gamma gamma1
+Hleng : Datatypes.length delta =? Datatypes.length delta1
+Halphad : all2 a_equiv_f (map snd delta) (map snd delta1)
+Halphagoal : a_equiv_f goal goal1
+______________________________________(1/1)
+errst_spec (st_wf (Some tsk1'))
+  (x <-
+   (f2 <- elim_let_rewrite f1;;
+    errst_ret
+      (change_tdecl_c tsk1'
+         (change_tdecl_node (task_decl tsk1') (Decl (change_decl_node d (Dprop (Pgoal, pr, f2)))))));;
+   errst_ret (Some x))
+  (fun (_ : full_st) (r : TaskDefs.task) (_ : full_st) =>
+   task_related r (gamma1, delta1, elim_let_f true true goal1)) *)
+
+(*tsk is initial task*)
+(*
+Lemma errst_spec_goal {St: Type} (tr: errState St TaskDefs.task) (fr: term_c -> errState St term_c) 
+  (f: formula -> formula)
+  (g1: term_c) (g2: formula) (Hgoal: eval_fmla g1 = Some g2)
+  P1 P2 (tsk: task_hd) gamma1 delta1
+  (Hg2: eval_task_goal tsk = Some g2)
+  (Hrel: task_related (Some tsk) tsk1)
+  (Hp12: forall s, P1 s -> P2 s):
+  (*condition: tr doesnt change context or hyps*)
+  errst_spec (fun _ => True) tr 
+    (fun _ r _ => exists (r': task_hd), r = Some r' /\ eval_task_ctx tsk = eval_task_ctx r' /\ 
+      eval_task_hyps tsk = eval_task_hyps r') ->
+  (*and tr changes goal to fr*)
+  (*TODO: not great that I don't use errst_spec but easier*)
+  (forall s1 b1 pr f1, fst (run_errState tr s1) = inr b1 -> find_goal (Some tsk) = Some (pr, f1) -> 
+      exists b2, fst (run_errState (fr g1) s1)= inr b2 /\
+       find_goal b1 = Some (pr, b2)) ->
+(*     exists pr f1, find_goal s1 = Some (pr, f1) -> find_goal b1 = Some 
+
+  errst_spec P1 tr (fun s1 r _ => forall pr f, find_goal s1 = Some (pr, f1) -> find_goal r = Some (pr, ) -> *)
+  errst_spec P2 (fr g1) (fun _ f2 _ => fmla_related f2 (f g2)) ->
+  errst_spec P1 tr (fun _ r _ => task_related r tsk1). (*Not tsk1, *)
+Proof.
+  (*This one we prove by unfolding*)
+  unfold errst_spec. intros Htr Htf Hfr i b Hp1 Hrun.
+  unfold task_related in *.
+  (*TODO: very wasteful to expand twice*)
+  destruct Hrel as [t1 [Heval Halpha]].
+  unfold eval_task in Heval.
+  apply option_bind_some in Heval.
+  destruct Heval as [gamma [Hgamma Heval]].
+  apply option_bind_some in Hgamma.
+  destruct Hgamma as [tsk1' [Hsome Hgamma]]. subst.
+  apply option_bind_some in Heval. simpl in Heval.
+  destruct Heval as [delta [Hdelta Heval]].
+  apply option_bind_some in Heval.
+  inversion Hsome; subst; clear Hsome.
+  destruct Heval as [goal1 [Hgoal1 Ht1]]. inversion Ht1; subst; clear Ht1.
+  rewrite Hg2 in Hgoal1. inversion Hgoal1; subst;clear Hgoal1.
+  (*Use assumptions and tr and fr*)
+  specialize (Htr i b I Hrun).
+  destruct b as [t|]; [|destruct_all; discriminate].
+  destruct Htr as [r' [Hr' [Hctx Hhyps]]]. inversion Hr'; subst; clear Hr'.
+  rewrite eval_task_find_goal in Hg2.
+  destruct Hg2 as [f1 [pr [Hfind Heval]]].
+
+ (*  unfold find_goal at 1 in Htf. simpl in Htf.
+  apply eval_task_find_goal 
+
+  unfold eval_task_goal, eval_tdecl_goal, eval_tdecl_node_aux, eval_decl_goal in Hg2.
+  unfold rewrite_goal.
+  destruct (td_node_of (task_decl tsk1')) as [d | | |] eqn : Htd; try discriminate.
+  unfold get_goal in Hgoal.
+  destruct (d_node d) as [| | | | | [[k pr] f1]] eqn : Hd; try discriminate.
+  simpl in *. destruct k; try discriminate. *)
+  specialize (Htf _ _ pr f1 Hrun Hfind).
+  destruct Htf as [b2 [Hb2 Hgoalr']].
+  specialize (Hfr _ _ (Hp12 _ Hp1) Hb2).
+  (*Now no more state monads*)
+  unfold fmla_related in Hfr. destruct Hfr as [f2 [Hevalb2 Halphaf]].
+  exists (gamma, delta, f2). split.
+  - unfold eval_task. simpl. rewrite <- Hctx, Hgamma. simpl.
+    rewrite <- Hhyps, Hdelta. simpl.
+    assert (Heval': eval_task_goal r' = Some f2).
+    {
+      apply eval_task_find_goal. exists b2. exists pr. split; auto.
+    }
+    rewrite Heval'. reflexivity.
+  - clear -Halpha Halphaf. (*TODO: make sure*) unfold a_equiv_task in *. 
+    destruct tsk1 as [[gamma1 delta1] goal1']. simpl_task.
+    bool_hyps. bool_to_prop; split_all; auto.
+    eapply a_equiv_f_trans. apply Halphaf.  
+    apply Alpha. *)
+
+
 (*The main part: prove related*)
-Theorem elim_let_related (tsk1 : task) (tsk2 : Task.task):
+Theorem elim_let_related (tsk1 : TaskDefs.task) (tsk2 : Task.task):
 errst_spec
   (fun s : full_st => st_wf tsk1 s /\ task_related tsk1 tsk2)
   (elim_let tsk1)
-  (fun (_ : full_st) (r : task) (_ : full_st) =>
+  (fun (_ : full_st) (r : TaskDefs.task) (_ : full_st) =>
    task_related r (single_goal (elim_let_f true true) tsk2)).
 Proof.
-  (*need to do induction on formula*)
-  (*Next steps:
-    1. prove we can move [task_related] out of condition (or maybe just change decomp?
-    2. unfold tasks, get elim_let and elim_let_f just on goal,
-      then need to get formulas, do induction on formulas
-      will need to reason about eval, related, and results via induction
-      do not want to unfold errst_spec if possible so we can prove intermediate results
-  unfold task_related at 1.
-  unfold errst_spec.
+  apply errst_spec_pure_pre.
+  intros Hrel.
 
 
+  (*Need to reason about goal formula*)
+  (*Lots of boilerplate to simplify tasks (TODO: separate lemma?)*)
+  unfold task_related in Hrel.
+  destruct Hrel as [t1 [Heval Halpha]].
+  unfold eval_task in Heval.
+  apply option_bind_some in Heval.
+  destruct Heval as [gamma [Hgamma Heval]].
+  apply option_bind_some in Hgamma.
+  destruct Hgamma as [tsk1' [Hsome Hgamma]]. subst.
+  apply option_bind_some in Heval. simpl in Heval.
+  destruct Heval as [delta [Hdelta Heval]].
+  apply option_bind_some in Heval.
+  destruct Heval as [goal [Hgoal Ht1]]. inversion Ht1; subst; clear Ht1.
+  destruct tsk2 as [[gamma1 delta1] goal1].
+  (*Now get info from [a_equiv_task]*)
+  unfold a_equiv_task in Halpha. simpl in Halpha. simpl_task.
+  rewrite !andb_true in Halpha.
+  destruct Halpha as [[[Halphag Hleng] Halphad] Halphagoal].
+  (*Now simplify elim_let (both) to reduce to goal *)
+  unfold single_goal. simpl_task.
+  unfold elim_let_aux.
+  (*Reduce to [rewrite_goal]*)
+  eapply prove_errst_spec_bnd with (Q1:=fun _ r _ => task_related (Some r) (gamma1, delta1, elim_let_f true true goal1))
+  (P2:=fun x _ => task_related (Some x)  (gamma1, delta1, elim_let_f true true goal1))
+  (Q2:= fun x _ y _ => task_related y  (gamma1, delta1, elim_let_f true true goal1)); auto.
+  2: { intros x. apply prove_errst_spec_ret. auto. }
+  (*Simplify [rewrite_goal] - could do separate lemma maybe*)
+  rewrite eval_task_find_goal in Hgoal. destruct Hgoal as [f1 [pr [Hfind Hevalf]]].
+  unfold find_goal in Hfind. simpl in Hfind. unfold rewrite_goal.
+  destruct (td_node_of (task_decl tsk1')) as [d | | |] eqn : Htd; try discriminate.
+  destruct (d_node d) as [| | | | | [[k pr1] f1']] eqn : Hd; try discriminate.
+  simpl in *. destruct k; try discriminate. inversion Hfind; subst; clear Hfind.
+  (*Now decompose bind again: first just gives us [elim_let_f goal], second
+    builds the task*)
+  (*TODO: think we will need to prove that result of [elim_let_f] is alpha equivalent*)
+  eapply prove_errst_spec_bnd with (Q1:=fun _ f2 _ => eval_fmla f2 = Some (elim_let_f true true goal))
+  (Q2:=fun x _ y _ => task_related (Some y) (gamma1, delta1, elim_let_f true true goal1))
+  (P2:=fun x _ => eval_fmla x = Some (elim_let_f true true goal)) (*TODO: see*); auto.
+  2: { (*Prove ending spec assuming [elim_let] correct*) intros f2. apply prove_errst_spec_ret. intros _ Hf2.
+    unfold task_related.
+    exists (gamma, delta, (elim_let_f true true goal)).
+    split.
+    - unfold eval_task. simpl.
+      (*TODO: prove these equal in separate lemmas for [change_*] lemmas since we change goal *)
+      admit.
+    - unfold a_equiv_task. simpl_task. bool_to_prop; split_all; auto.
+      (*TODO: prove that a_equiv_f preserved by elim_let_f*)
+      admit.
+  }
+  (*TODO: prove that these transformations related. NOTE: everything up to now wasnt super
+    specific to [elim_let] and it could/should be refactored*)
+  (*TODO: weaken precondition and use separate lemma*)
+Admitted.
 
 
 Theorem elim_let_sound: trans_errst_sound elim_let.
 Proof.
   apply prove_trans_errst_decompose with (tr1:=single_goal (elim_let_f true true)).
   - (*already proved soundness*) apply elim_let_sound. 
-  - (*Now prove related*)
+  - (*Now prove related*) apply elim_let_related.
+Qed.
 
 
